
Correction Exercice 1

$A=(x+5)^2\\=x^2+2\times 5 \times x+5^2\\=x^2+10x+25$

$B=(x-3)^2\\=x^2-2\times 3\times x+3^2\\=x^2-6x+9$

$C=(x+4)(x-4)\\=x^2-4^2\\=x^2-16$

$D=(x+7)^2\\=x^2+2\times 7\times x+7^2\\=x^2+14x+49$

$E=(x-1)^2\\=x^2-2\times 1\times x+1^2\\=x^2-2x+1$

$F=(x-6)(x+6)\\=x^2-6^2\\=x^2-36$

Correction Exercice 2

$A=(2x+3)^2\\=(2x)^2+2\times 3\times 2x+3^2\\=4x^2+12x+9$

$B=(5x-4)^2\\=(5x)^2-2\times 4\times 5x+4^2\\=25x^2-40x+16$

$C=(3x-2)(3x+2)\\=(3x)^2-2^2\\=9x^2-4$

$D=(6-3x)^2\\=6^2-2\times 6\times 3x+(3x)^2\\=36-36x+9x^2$

$E=(1+8x)^2\\=1^2+2\times 1\times 8x+(8x)^2\\=1+16x+64x^2$

$F=(4x+5)(5-4x)\\=(5+4x)(5-4x)\\=5^2-(4x)^2\\=25-16x^2$

Correction Exercice 3

$ A=(4x+3)^2 \\
=(4x)^2+2\times 4x\times 3+3^2 \\
=16x^2+24x+9
$

$ B=(6x-7)^2 \\
=(6x)^2-2\times 6x \times 7 + 7^2 \\
=36x^2-84x+49
$

$C=(5x+4)(5x-4) \\
=(5x)^2-4^2 \\
=25x^2-16
$

$ D=(3x+7)^2 \\
=(3x)^2+2\times 3x \times 7 + 7^2 \\
=9x^2+42x+49
$

$ E=(7x-5)^2 \\
=(7x)^2-2\times 7x \times 5+5^2 \\
=49x^2-70x+25
$

$ F=(3x-5)(3x+5) \\
=(3x)^2-5^2 \\
=9x^2-25
$

$ G=(7-4x)^2 \\
=7^2-2\times 7 \times 4x + (4x)^2 \\
=49-56x+16x^2
$

$ H=(2x+9)^2 \\
=(2x)^2+2\times 2x \times 9 + 9^2 \\
=4x^2+36x+81
$

$ I=(6-2x)(6+2x) \\
=6^2-(2x)^2 \\
=36-4x^2
$

Correction Exercice 4

$ A=\left(x+\dfrac{1}{3}\right)^2 \\
=x^2+2 \times x\times \dfrac{1}{3} + \left(\dfrac{1}{3}\right)^2 \\
=x^2+\dfrac{2}{3}x + \dfrac{1}{9}
$

$ B=\left(2x-\dfrac{1}{2}\right)^2 \\
=(2x)^2-2\times 2x \times \dfrac{1}{2}+\left(\dfrac{1}{2}\right)^2 \\
=4x^2-2x+\dfrac{1}{4}
$

$ C=\left(6x+\dfrac{2}{5}\right)\left(6x-\dfrac{2}{5}\right) \\
=(6x)^2-\left(\dfrac{2}{5}\right)^2 \\
=36x^2-\dfrac{4}{25}
$

$D=\left(3x+\dfrac{7}{6}\right)^2 \\
=(3x)^2+2\times 3x \times \dfrac{7}{6}+\left(\dfrac{7}{6}\right)^2 \\
=9x^2+7x+\dfrac{49}{36}
$

$ E=\left(3x-\dfrac{4}{3}\right)^2 \\
=(3x)^2-2\times 3x \times \dfrac{4}{3}+\left(\dfrac{4}{3}\right)^2 \\
=9x^2-8x+\dfrac{16}{9}
$

$F=\left(\dfrac{7}{4}x+\dfrac{1}{2}\right)\left(\dfrac{7}{4}x-\dfrac{1}{2}\right) \\
=\left(\dfrac{7}{4}x\right)^2-\left(\dfrac{1}{2}\right)^2 \\
=\dfrac{49}{16}x^2-\dfrac{1}{4}
$

$ G=\left(2x-\dfrac{5}{2}\right)^2 \\
=(2x)^2-2\times 2x\times \dfrac{5}{2}+\left(\dfrac{5}{2}\right)^2 \\
=4x^2-10x+\dfrac{25}{4}
$

$H=\left(3x-\dfrac{7}{3}\right)^2 \\
=(3x)^2-2\times 3x\times \dfrac{7}{3}+\left(\dfrac{7}{3}\right)^2 \\
=9x^2-14x+\dfrac{49}{9}
$

Correction Exercice 5

$A=(2x+5)^2-(3x-4)^2\\
=(2x)^2+2\times 5\times 2x+5^2-\left((3x)^2-2\times 3x\times 4+ 4^2\right) \\
=4x^2+20x+25-\left(9x^2-24x+16\right) \\
=4x^2+20x+25-9x^2+24x-16\\
=-5x^2+44x+9$

$B=(5x+7)^2+(2x-6)^2\\
=(5x)^2+2\times 7\times 5x+7^2+(2x)^2-2\times 6\times 2x+6^2\\
=25x^2+70x+49+4x^2-24x+36\\
=29x^2+46x+85$

$C=(7x+2)^2-(4x-3)(4x+3) \\
=(7x)^2+2\times 2\times 7x+2^2-\left((4x)^2-3^2\right) \\
=49x^2+28x+4-\left(16x^2-9\right) \\
=49x^2+28x+4-16x^2+9\\
=33x^2+28x+13$

$D=(3x-5)(3x+5)-(3x+5)^2\\
=(3x)^2-5^2-\left((3x)^2+2\times 5\times 3x+5^2\right) \\
=9x^2-25-\left(9x^2+30x+25\right) \\
=9x^2-25-9x^2-30x-25\\
=-30x-50$

$E=(5x-3)^2-(3x-7)^2\\
=(5x)^2-2\times 3\times 5x+3^2-\left((3x)^2-2\times 7\times 3x+7^2\right) \\
=25x^2-30x+9-\left(9x^2-42x+49\right) \\
=25x^2-30x+9-9x^2+42x-49\\
=16x^2+12x-40$

$F=(7x-3)(7x+3)-(8x+5)(8x-5) \\
=(7x)^2-3^2-\left((8x)^2-5^2\right) \\
=49x^2-9-\left(64x^2-25\right) \\
=49x^2-9-64x^2+25\\
=-15x^2+16
$

